floyd/funspec_old.v
@@ -22,106 +22,106 @@ Notation " a 'OF' ta " := (a%positive,ta%type) (at level 100, only parsing): for
 Delimit Scope formals with formals.
 
 Notation "'WITH' x : tx 'PRE'  [ u , .. , v ] P 'POST' [ tz ] Q" :=
-     (NDmk_funspec ((cons u%formals .. (cons v%formals nil) ..), tz) cc_default tx (fun x => P%assert) (fun x => Q%assert))
+     (mk_funspec' ((cons u%formals .. (cons v%formals nil) ..), tz) cc_default tx (fun x => P%assert) (fun x => Q%assert))
             (at level 200, x at level 0, P at level 100, Q at level 100) : old_funspec_scope.
 
 Notation "'WITH' x : tx 'PRE'  [ ] P 'POST' [ tz ] Q" :=
-     (NDmk_funspec (nil, tz) cc_default tx (fun x => P%assert) (fun x => Q%assert))
+     (mk_funspec' (nil, tz) cc_default tx (fun x => P%assert) (fun x => Q%assert))
             (at level 200, x at level 0, P at level 100, Q at level 100) : old_funspec_scope.
 
 Notation "'WITH'  x1 : t1 , x2 : t2 'PRE'  [ u , .. , v ] P 'POST' [ tz ] Q" :=
-     (NDmk_funspec ((cons u%formals .. (cons v%formals nil) ..), tz) cc_default (t1*t2)
+     (mk_funspec' ((cons u%formals .. (cons v%formals nil) ..), tz) cc_default (t1*t2)
            (fun x => match x with (x1,x2) => P%assert end)
            (fun x => match x with (x1,x2) => Q%assert end))
             (at level 200, x1 at level 0, x2 at level 0, P at level 100, Q at level 100) : old_funspec_scope.
 
 Notation "'WITH'  x1 : t1 , x2 : t2 'PRE'  [ ] P 'POST' [ tz ] Q" :=
-     (NDmk_funspec (nil, tz) cc_default (t1*t2)
+     (mk_funspec' (nil, tz) cc_default (t1*t2)
            (fun x => match x with (x1,x2) => P%assert end)
            (fun x => match x with (x1,x2) => Q%assert end))
             (at level 200, x1 at level 0, x2 at level 0, P at level 100, Q at level 100) : old_funspec_scope.
 
 Notation "'WITH'  x1 : t1 , x2 : t2 , x3 : t3 'PRE'  [ u , .. , v ] P 'POST' [ tz ] Q" :=
-     (NDmk_funspec ((cons u%formals .. (cons v%formals nil) ..), tz) cc_default (t1*t2*t3)
+     (mk_funspec' ((cons u%formals .. (cons v%formals nil) ..), tz) cc_default (t1*t2*t3)
            (fun x => match x with (x1,x2,x3) => P%assert end)
            (fun x => match x with (x1,x2,x3) => Q%assert end))
             (at level 200, x1 at level 0, x2 at level 0, x3 at level 0, P at level 100, Q at level 100) : old_funspec_scope.
 
 Notation "'WITH'  x1 : t1 , x2 : t2 , x3 : t3 'PRE'  [ ] P 'POST' [ tz ] Q" :=
-     (NDmk_funspec (nil, tz) cc_default (t1*t2*t3)
+     (mk_funspec' (nil, tz) cc_default (t1*t2*t3)
            (fun x => match x with (x1,x2,x3) => P%assert end)
            (fun x => match x with (x1,x2,x3) => Q%assert end))
             (at level 200, x1 at level 0, x2 at level 0, x3 at level 0, P at level 100, Q at level 100) : old_funspec_scope.
 
 
 Notation "'WITH'  x1 : t1 , x2 : t2 , x3 : t3 , x4 : t4 'PRE'  [ u , .. , v ] P 'POST' [ tz ] Q" :=
-     (NDmk_funspec ((cons u%formals .. (cons v%formals nil) ..), tz) cc_default (t1*t2*t3*t4)
+     (mk_funspec' ((cons u%formals .. (cons v%formals nil) ..), tz) cc_default (t1*t2*t3*t4)
            (fun x => match x with (x1,x2,x3,x4) => P%assert end)
            (fun x => match x with (x1,x2,x3,x4) => Q%assert end))
             (at level 200, x1 at level 0, x2 at level 0, x3 at level 0, x4 at level 0, P at level 100, Q at level 100) : old_funspec_scope.
 
 Notation "'WITH'  x1 : t1 , x2 : t2 , x3 : t3 , x4 : t4 'PRE'  [ ] P 'POST' [ tz ] Q" :=
-     (NDmk_funspec (nil, tz) cc_default (t1*t2*t3*t4)
+     (mk_funspec' (nil, tz) cc_default (t1*t2*t3*t4)
            (fun x => match x with (x1,x2,x3,x4) => P%assert end)
            (fun x => match x with (x1,x2,x3,x4) => Q%assert end))
             (at level 200, x1 at level 0, x2 at level 0, x3 at level 0, x4 at level 0, P at level 100, Q at level 100) : old_funspec_scope.
 
 Notation "'WITH'  x1 : t1 , x2 : t2 , x3 : t3 , x4 : t4 , x5 : t5 'PRE'  [ ] P 'POST' [ tz ] Q" :=
-     (NDmk_funspec (nil, tz) cc_default (t1*t2*t3*t4*t5)
+     (mk_funspec' (nil, tz) cc_default (t1*t2*t3*t4*t5)
            (fun x => match x with (x1,x2,x3,x4,x5) => P%assert end)
            (fun x => match x with (x1,x2,x3,x4,x5) => Q%assert end))
             (at level 200, x1 at level 0, x2 at level 0, x3 at level 0, x4 at level 0, x5 at level 0, P at level 100, Q at level 100) : old_funspec_scope.
 
 Notation "'WITH'  x1 : t1 , x2 : t2 , x3 : t3 , x4 : t4 , x5 : t5 'PRE'  [ u , .. , v ] P 'POST' [ tz ] Q" :=
-     (NDmk_funspec ((cons u%formals .. (cons v%formals nil) ..), tz) cc_default (t1*t2*t3*t4*t5)
+     (mk_funspec' ((cons u%formals .. (cons v%formals nil) ..), tz) cc_default (t1*t2*t3*t4*t5)
            (fun x => match x with (x1,x2,x3,x4,x5) => P%assert end)
            (fun x => match x with (x1,x2,x3,x4,x5) => Q%assert end))
             (at level 200, x1 at level 0, x2 at level 0, x3 at level 0, x4 at level 0, x5 at level 0, P at level 100, Q at level 100) : old_funspec_scope.
 
 Notation "'WITH'  x1 : t1 , x2 : t2 , x3 : t3 , x4 : t4 , x5 : t5 , x6 : t6 'PRE'  [ ] P 'POST' [ tz ] Q" :=
-     (NDmk_funspec (nil, tz) cc_default (t1*t2*t3*t4*t5*t6)
+     (mk_funspec' (nil, tz) cc_default (t1*t2*t3*t4*t5*t6)
            (fun x => match x with (x1,x2,x3,x4,x5,x6) => P%assert end)
            (fun x => match x with (x1,x2,x3,x4,x5,x6) => Q%assert end))
             (at level 200, x1 at level 0, x2 at level 0, x3 at level 0, x4 at level 0,
               x5 at level 0, x6 at level 0, P at level 100, Q at level 100) : old_funspec_scope.
 
 Notation "'WITH'  x1 : t1 , x2 : t2 , x3 : t3 , x4 : t4 , x5 : t5 , x6 : t6 'PRE'  [ u , .. , v ] P 'POST' [ tz ] Q" :=
-     (NDmk_funspec ((cons u%formals .. (cons v%formals nil) ..), tz) cc_default (t1*t2*t3*t4*t5*t6)
+     (mk_funspec' ((cons u%formals .. (cons v%formals nil) ..), tz) cc_default (t1*t2*t3*t4*t5*t6)
            (fun x => match x with (x1,x2,x3,x4,x5,x6) => P%assert end)
            (fun x => match x with (x1,x2,x3,x4,x5,x6) => Q%assert end))
             (at level 200, x1 at level 0, x2 at level 0, x3 at level 0, x4 at level 0,
              x5 at level 0, x6 at level 0, P at level 100, Q at level 100) : old_funspec_scope.
 
 Notation "'WITH'  x1 : t1 , x2 : t2 , x3 : t3 , x4 : t4 , x5 : t5 , x6 : t6 , x7 : t7 'PRE'  [ ] P 'POST' [ tz ] Q" :=
-     (NDmk_funspec (nil, tz) cc_default (t1*t2*t3*t4*t5*t6*t7)
+     (mk_funspec' (nil, tz) cc_default (t1*t2*t3*t4*t5*t6*t7)
            (fun x => match x with (x1,x2,x3,x4,x5,x6,x7) => P%assert end)
            (fun x => match x with (x1,x2,x3,x4,x5,x6,x7) => Q%assert end))
             (at level 200, x1 at level 0, x2 at level 0, x3 at level 0, x4 at level 0,
               x5 at level 0, x6 at level 0, x7 at level 0, P at level 100, Q at level 100) : old_funspec_scope.
 
 Notation "'WITH'  x1 : t1 , x2 : t2 , x3 : t3 , x4 : t4 , x5 : t5 , x6 : t6 , x7 : t7 'PRE'  [ u , .. , v ] P 'POST' [ tz ] Q" :=
-     (NDmk_funspec ((cons u%formals .. (cons v%formals nil) ..), tz) cc_default (t1*t2*t3*t4*t5*t6*t7)
+     (mk_funspec' ((cons u%formals .. (cons v%formals nil) ..), tz) cc_default (t1*t2*t3*t4*t5*t6*t7)
            (fun x => match x with (x1,x2,x3,x4,x5,x6,x7) => P%assert end)
            (fun x => match x with (x1,x2,x3,x4,x5,x6,x7) => Q%assert end))
             (at level 200, x1 at level 0, x2 at level 0, x3 at level 0, x4 at level 0,
              x5 at level 0, x6 at level 0, x7 at level 0, P at level 100, Q at level 100) : old_funspec_scope.
 
 Notation "'WITH'  x1 : t1 , x2 : t2 , x3 : t3 , x4 : t4 , x5 : t5 , x6 : t6 , x7 : t7 , x8 : t8 'PRE'  [ ] P 'POST' [ tz ] Q" :=
-     (NDmk_funspec (nil, tz) cc_default (t1*t2*t3*t4*t5*t6*t7*t8)
+     (mk_funspec' (nil, tz) cc_default (t1*t2*t3*t4*t5*t6*t7*t8)
            (fun x => match x with (x1,x2,x3,x4,x5,x6,x7,x8) => P%assert end)
            (fun x => match x with (x1,x2,x3,x4,x5,x6,x7,x8) => Q%assert end))
             (at level 200, x1 at level 0, x2 at level 0, x3 at level 0, x4 at level 0,
               x5 at level 0, x6 at level 0, x7 at level 0, x8 at level 0, P at level 100, Q at level 100) : old_funspec_scope.
 
 Notation "'WITH'  x1 : t1 , x2 : t2 , x3 : t3 , x4 : t4 , x5 : t5 , x6 : t6 , x7 : t7 , x8 : t8 'PRE'  [ u , .. , v ] P 'POST' [ tz ] Q" :=
-     (NDmk_funspec ((cons u%formals .. (cons v%formals nil) ..), tz) cc_default (t1*t2*t3*t4*t5*t6*t7*t8)
+     (mk_funspec' ((cons u%formals .. (cons v%formals nil) ..), tz) cc_default (t1*t2*t3*t4*t5*t6*t7*t8)
            (fun x => match x with (x1,x2,x3,x4,x5,x6,x7,x8) => P%assert end)
            (fun x => match x with (x1,x2,x3,x4,x5,x6,x7,x8) => Q%assert end))
             (at level 200, x1 at level 0, x2 at level 0, x3 at level 0, x4 at level 0,
              x5 at level 0, x6 at level 0, x7 at level 0, x8 at level 0, P at level 100, Q at level 100) : old_funspec_scope.
 
 Notation "'WITH'  x1 : t1 , x2 : t2 , x3 : t3 , x4 : t4 , x5 : t5 , x6 : t6 , x7 : t7 , x8 : t8 , x9 : t9 'PRE'  [ ] P 'POST' [ tz ] Q" :=
-     (NDmk_funspec (nil, tz) cc_default (t1*t2*t3*t4*t5*t6*t7*t8*t9)
+     (mk_funspec' (nil, tz) cc_default (t1*t2*t3*t4*t5*t6*t7*t8*t9)
            (fun x => match x with (x1,x2,x3,x4,x5,x6,x7,x8,x9) => P%assert end)
            (fun x => match x with (x1,x2,x3,x4,x5,x6,x7,x8,x9) => Q%assert end))
             (at level 200, x1 at level 0, x2 at level 0, x3 at level 0, x4 at level 0,
@@ -129,7 +129,7 @@ Notation "'WITH'  x1 : t1 , x2 : t2 , x3 : t3 , x4 : t4 , x5 : t5 , x6 : t6 , x7
              P at level 100, Q at level 100) : old_funspec_scope.
 
 Notation "'WITH'  x1 : t1 , x2 : t2 , x3 : t3 , x4 : t4 , x5 : t5 , x6 : t6 , x7 : t7 , x8 : t8 , x9 : t9 'PRE'  [ u , .. , v ] P 'POST' [ tz ] Q" :=
-     (NDmk_funspec ((cons u%formals .. (cons v%formals nil) ..), tz) cc_default (t1*t2*t3*t4*t5*t6*t7*t8*t9)
+     (mk_funspec' ((cons u%formals .. (cons v%formals nil) ..), tz) cc_default (t1*t2*t3*t4*t5*t6*t7*t8*t9)
            (fun x => match x with (x1,x2,x3,x4,x5,x6,x7,x8,x9) => P%assert end)
            (fun x => match x with (x1,x2,x3,x4,x5,x6,x7,x8,x9) => Q%assert end))
             (at level 200, x1 at level 0, x2 at level 0, x3 at level 0, x4 at level 0,
@@ -137,7 +137,7 @@ Notation "'WITH'  x1 : t1 , x2 : t2 , x3 : t3 , x4 : t4 , x5 : t5 , x6 : t6 , x7
              P at level 100, Q at level 100) : old_funspec_scope.
 
 Notation "'WITH'  x1 : t1 , x2 : t2 , x3 : t3 , x4 : t4 , x5 : t5 , x6 : t6 , x7 : t7 , x8 : t8 , x9 : t9 , x10 : t10 'PRE'  [ ] P 'POST' [ tz ] Q" :=
-     (NDmk_funspec (nil, tz) cc_default (t1*t2*t3*t4*t5*t6*t7*t8*t9*t10)
+     (mk_funspec' (nil, tz) cc_default (t1*t2*t3*t4*t5*t6*t7*t8*t9*t10)
            (fun x => match x with (x1,x2,x3,x4,x5,x6,x7,x8,x9,x10) => P%assert end)
            (fun x => match x with (x1,x2,x3,x4,x5,x6,x7,x8,x9,x10) => Q%assert end))
             (at level 200, x1 at level 0, x2 at level 0, x3 at level 0, x4 at level 0,
@@ -146,7 +146,7 @@ Notation "'WITH'  x1 : t1 , x2 : t2 , x3 : t3 , x4 : t4 , x5 : t5 , x6 : t6 , x7
              P at level 100, Q at level 100) : old_funspec_scope.
 
 Notation "'WITH'  x1 : t1 , x2 : t2 , x3 : t3 , x4 : t4 , x5 : t5 , x6 : t6 , x7 : t7 , x8 : t8 , x9 : t9 , x10 : t10 'PRE'  [ u , .. , v ] P 'POST' [ tz ] Q" :=
-     (NDmk_funspec ((cons u%formals .. (cons v%formals nil) ..), tz) cc_default (t1*t2*t3*t4*t5*t6*t7*t8*t9*t10)
+     (mk_funspec' ((cons u%formals .. (cons v%formals nil) ..), tz) cc_default (t1*t2*t3*t4*t5*t6*t7*t8*t9*t10)
            (fun x => match x with (x1,x2,x3,x4,x5,x6,x7,x8,x9,x10) => P%assert end)
            (fun x => match x with (x1,x2,x3,x4,x5,x6,x7,x8,x9,x10) => Q%assert end))
             (at level 200, x1 at level 0, x2 at level 0, x3 at level 0, x4 at level 0,
@@ -155,7 +155,7 @@ Notation "'WITH'  x1 : t1 , x2 : t2 , x3 : t3 , x4 : t4 , x5 : t5 , x6 : t6 , x7
              P at level 100, Q at level 100) : old_funspec_scope.
 
 Notation "'WITH'  x1 : t1 , x2 : t2 , x3 : t3 , x4 : t4 , x5 : t5 , x6 : t6 , x7 : t7 , x8 : t8 , x9 : t9 , x10 : t10 , x11 : t11 'PRE'  [ ] P 'POST' [ tz ] Q" :=
-     (NDmk_funspec (nil, tz) cc_default (t1*t2*t3*t4*t5*t6*t7*t8*t9*t10*t11)
+     (mk_funspec' (nil, tz) cc_default (t1*t2*t3*t4*t5*t6*t7*t8*t9*t10*t11)
            (fun x => match x with (x1,x2,x3,x4,x5,x6,x7,x8,x9,x10,x11) => P%assert end)
            (fun x => match x with (x1,x2,x3,x4,x5,x6,x7,x8,x9,x10,x11) => Q%assert end))
             (at level 200, x1 at level 0, x2 at level 0, x3 at level 0, x4 at level 0,
@@ -164,7 +164,7 @@ Notation "'WITH'  x1 : t1 , x2 : t2 , x3 : t3 , x4 : t4 , x5 : t5 , x6 : t6 , x7
              P at level 100, Q at level 100) : old_funspec_scope.
 
 Notation "'WITH'  x1 : t1 , x2 : t2 , x3 : t3 , x4 : t4 , x5 : t5 , x6 : t6 , x7 : t7 , x8 : t8 , x9 : t9 , x10 : t10 , x11 : t11 'PRE'  [ u , .. , v ] P 'POST' [ tz ] Q" :=
-     (NDmk_funspec ((cons u%formals .. (cons v%formals nil) ..), tz) cc_default (t1*t2*t3*t4*t5*t6*t7*t8*t9*t10*t11)
+     (mk_funspec' ((cons u%formals .. (cons v%formals nil) ..), tz) cc_default (t1*t2*t3*t4*t5*t6*t7*t8*t9*t10*t11)
            (fun x => match x with (x1,x2,x3,x4,x5,x6,x7,x8,x9,x10,x11) => P%assert end)
            (fun x => match x with (x1,x2,x3,x4,x5,x6,x7,x8,x9,x10,x11) => Q%assert end))
             (at level 200, x1 at level 0, x2 at level 0, x3 at level 0, x4 at level 0,
@@ -173,7 +173,7 @@ Notation "'WITH'  x1 : t1 , x2 : t2 , x3 : t3 , x4 : t4 , x5 : t5 , x6 : t6 , x7
              P at level 100, Q at level 100) : old_funspec_scope.
 
 Notation "'WITH'  x1 : t1 , x2 : t2 , x3 : t3 , x4 : t4 , x5 : t5 , x6 : t6 , x7 : t7 , x8 : t8 , x9 : t9 , x10 : t10 , x11 : t11 , x12 : t12 'PRE'  [ ] P 'POST' [ tz ] Q" :=
-     (NDmk_funspec (nil, tz) cc_default (t1*t2*t3*t4*t5*t6*t7*t8*t9*t10*t11*t12)
+     (mk_funspec' (nil, tz) cc_default (t1*t2*t3*t4*t5*t6*t7*t8*t9*t10*t11*t12)
            (fun x => match x with (x1,x2,x3,x4,x5,x6,x7,x8,x9,x10,x11,x12) => P%assert end)
            (fun x => match x with (x1,x2,x3,x4,x5,x6,x7,x8,x9,x10,x11,x12) => Q%assert end))
             (at level 200, x1 at level 0, x2 at level 0, x3 at level 0, x4 at level 0,
@@ -182,7 +182,7 @@ Notation "'WITH'  x1 : t1 , x2 : t2 , x3 : t3 , x4 : t4 , x5 : t5 , x6 : t6 , x7
              P at level 100, Q at level 100) : old_funspec_scope.
 
 Notation "'WITH'  x1 : t1 , x2 : t2 , x3 : t3 , x4 : t4 , x5 : t5 , x6 : t6 , x7 : t7 , x8 : t8 , x9 : t9 , x10 : t10 , x11 : t11 , x12 : t12 'PRE'  [ u , .. , v ] P 'POST' [ tz ] Q" :=
-     (NDmk_funspec ((cons u%formals .. (cons v%formals nil) ..), tz) cc_default (t1*t2*t3*t4*t5*t6*t7*t8*t9*t10*t11*t12)
+     (mk_funspec' ((cons u%formals .. (cons v%formals nil) ..), tz) cc_default (t1*t2*t3*t4*t5*t6*t7*t8*t9*t10*t11*t12)
            (fun x => match x with (x1,x2,x3,x4,x5,x6,x7,x8,x9,x10,x11,x12) => P%assert end)
            (fun x => match x with (x1,x2,x3,x4,x5,x6,x7,x8,x9,x10,x11,x12) => Q%assert end))
             (at level 200, x1 at level 0, x2 at level 0, x3 at level 0, x4 at level 0,
@@ -191,7 +191,7 @@ Notation "'WITH'  x1 : t1 , x2 : t2 , x3 : t3 , x4 : t4 , x5 : t5 , x6 : t6 , x7
              P at level 100, Q at level 100) : old_funspec_scope.
 
 Notation "'WITH'  x1 : t1 , x2 : t2 , x3 : t3 , x4 : t4 , x5 : t5 , x6 : t6 , x7 : t7 , x8 : t8 , x9 : t9 , x10 : t10 , x11 : t11 , x12 : t12 , x13 : t13 'PRE'  [ ] P 'POST' [ tz ] Q" :=
-     (NDmk_funspec (nil, tz) cc_default (t1*t2*t3*t4*t5*t6*t7*t8*t9*t10*t11*t12*t13)
+     (mk_funspec' (nil, tz) cc_default (t1*t2*t3*t4*t5*t6*t7*t8*t9*t10*t11*t12*t13)
            (fun x => match x with (x1,x2,x3,x4,x5,x6,x7,x8,x9,x10,x11,x12,x13) => P%assert end)
            (fun x => match x with (x1,x2,x3,x4,x5,x6,x7,x8,x9,x10,x11,x12,x13) => Q%assert end))
             (at level 200, x1 at level 0, x2 at level 0, x3 at level 0, x4 at level 0,
@@ -200,7 +200,7 @@ Notation "'WITH'  x1 : t1 , x2 : t2 , x3 : t3 , x4 : t4 , x5 : t5 , x6 : t6 , x7
              P at level 100, Q at level 100) : old_funspec_scope.
 
 Notation "'WITH'  x1 : t1 , x2 : t2 , x3 : t3 , x4 : t4 , x5 : t5 , x6 : t6 , x7 : t7 , x8 : t8 , x9 : t9 , x10 : t10 , x11 : t11 , x12 : t12 , x13 : t13 'PRE'  [ u , .. , v ] P 'POST' [ tz ] Q" :=
-     (NDmk_funspec ((cons u%formals .. (cons v%formals nil) ..), tz) cc_default (t1*t2*t3*t4*t5*t6*t7*t8*t9*t10*t11*t12*t13)
+     (mk_funspec' ((cons u%formals .. (cons v%formals nil) ..), tz) cc_default (t1*t2*t3*t4*t5*t6*t7*t8*t9*t10*t11*t12*t13)
            (fun x => match x with (x1,x2,x3,x4,x5,x6,x7,x8,x9,x10,x11,x12,x13) => P%assert end)
            (fun x => match x with (x1,x2,x3,x4,x5,x6,x7,x8,x9,x10,x11,x12,x13) => Q%assert end))
             (at level 200, x1 at level 0, x2 at level 0, x3 at level 0, x4 at level 0,
@@ -209,7 +209,7 @@ Notation "'WITH'  x1 : t1 , x2 : t2 , x3 : t3 , x4 : t4 , x5 : t5 , x6 : t6 , x7
              P at level 100, Q at level 100) : old_funspec_scope.
 
 Notation "'WITH'  x1 : t1 , x2 : t2 , x3 : t3 , x4 : t4 , x5 : t5 , x6 : t6 , x7 : t7 , x8 : t8 , x9 : t9 , x10 : t10 , x11 : t11 , x12 : t12 , x13 : t13 , x14 : t14 'PRE'  [ ] P 'POST' [ tz ] Q" :=
-     (NDmk_funspec (nil, tz) cc_default (t1*t2*t3*t4*t5*t6*t7*t8*t9*t10*t11*t12*t13*t14)
+     (mk_funspec' (nil, tz) cc_default (t1*t2*t3*t4*t5*t6*t7*t8*t9*t10*t11*t12*t13*t14)
            (fun x => match x with (x1,x2,x3,x4,x5,x6,x7,x8,x9,x10,x11,x12,x13,x14) => P%assert end)
            (fun x => match x with (x1,x2,x3,x4,x5,x6,x7,x8,x9,x10,x11,x12,x13,x14) => Q%assert end))
             (at level 200, x1 at level 0, x2 at level 0, x3 at level 0, x4 at level 0,
@@ -218,7 +218,7 @@ Notation "'WITH'  x1 : t1 , x2 : t2 , x3 : t3 , x4 : t4 , x5 : t5 , x6 : t6 , x7
              P at level 100, Q at level 100) : old_funspec_scope.
 
 Notation "'WITH'  x1 : t1 , x2 : t2 , x3 : t3 , x4 : t4 , x5 : t5 , x6 : t6 , x7 : t7 , x8 : t8 , x9 : t9 , x10 : t10 , x11 : t11 , x12 : t12 , x13 : t13 , x14 : t14 'PRE'  [ u , .. , v ] P 'POST' [ tz ] Q" :=
-     (NDmk_funspec ((cons u%formals .. (cons v%formals nil) ..), tz) cc_default (t1*t2*t3*t4*t5*t6*t7*t8*t9*t10*t11*t12*t13*t14)
+     (mk_funspec' ((cons u%formals .. (cons v%formals nil) ..), tz) cc_default (t1*t2*t3*t4*t5*t6*t7*t8*t9*t10*t11*t12*t13*t14)
            (fun x => match x with (x1,x2,x3,x4,x5,x6,x7,x8,x9,x10,x11,x12,x13,x14) => P%assert end)
            (fun x => match x with (x1,x2,x3,x4,x5,x6,x7,x8,x9,x10,x11,x12,x13,x14) => Q%assert end))
             (at level 200, x1 at level 0, x2 at level 0, x3 at level 0, x4 at level 0,
@@ -227,7 +227,7 @@ Notation "'WITH'  x1 : t1 , x2 : t2 , x3 : t3 , x4 : t4 , x5 : t5 , x6 : t6 , x7
              P at level 100, Q at level 100) : old_funspec_scope.
 
 Notation "'WITH'  x1 : t1 , x2 : t2 , x3 : t3 , x4 : t4 , x5 : t5 , x6 : t6 , x7 : t7 , x8 : t8 , x9 : t9 , x10 : t10 , x11 : t11 , x12 : t12 , x13 : t13 , x14 : t14 , x15 : t15 'PRE'  [ ] P 'POST' [ tz ] Q" :=
-     (NDmk_funspec (nil, tz) cc_default (t1*t2*t3*t4*t5*t6*t7*t8*t9*t10*t11*t12*t13*t14*t15)
+     (mk_funspec' (nil, tz) cc_default (t1*t2*t3*t4*t5*t6*t7*t8*t9*t10*t11*t12*t13*t14*t15)
            (fun x => match x with (x1,x2,x3,x4,x5,x6,x7,x8,x9,x10,x11,x12,x13,x14,x15) => P%assert end)
            (fun x => match x with (x1,x2,x3,x4,x5,x6,x7,x8,x9,x10,x11,x12,x13,x14,x15) => Q%assert end))
             (at level 200, x1 at level 0, x2 at level 0, x3 at level 0, x4 at level 0,
@@ -238,7 +238,7 @@ Notation "'WITH'  x1 : t1 , x2 : t2 , x3 : t3 , x4 : t4 , x5 : t5 , x6 : t6 , x7
 
 
 Notation "'WITH'  x1 : t1 , x2 : t2 , x3 : t3 , x4 : t4 , x5 : t5 , x6 : t6 , x7 : t7 , x8 : t8 , x9 : t9 , x10 : t10 , x11 : t11 , x12 : t12 , x13 : t13 , x14 : t14 , x15 : t15 'PRE'  [ u , .. , v ] P 'POST' [ tz ] Q" :=
-     (NDmk_funspec ((cons u%formals .. (cons v%formals nil) ..), tz) cc_default (t1*t2*t3*t4*t5*t6*t7*t8*t9*t10*t11*t12*t13*t14*t15)
+     (mk_funspec' ((cons u%formals .. (cons v%formals nil) ..), tz) cc_default (t1*t2*t3*t4*t5*t6*t7*t8*t9*t10*t11*t12*t13*t14*t15)
            (fun x => match x with (x1,x2,x3,x4,x5,x6,x7,x8,x9,x10,x11,x12,x13,x14,x15) => P%assert end)
            (fun x => match x with (x1,x2,x3,x4,x5,x6,x7,x8,x9,x10,x11,x12,x13,x14,x15) => Q%assert end))
             (at level 200, x1 at level 0, x2 at level 0, x3 at level 0, x4 at level 0,
@@ -248,7 +248,7 @@ Notation "'WITH'  x1 : t1 , x2 : t2 , x3 : t3 , x4 : t4 , x5 : t5 , x6 : t6 , x7
              P at level 100, Q at level 100) : old_funspec_scope.
 
 Notation "'WITH'  x1 : t1 , x2 : t2 , x3 : t3 , x4 : t4 , x5 : t5 , x6 : t6 , x7 : t7 , x8 : t8 , x9 : t9 , x10 : t10 , x11 : t11 , x12 : t12 , x13 : t13 , x14 : t14 , x15 : t15 , x16 : t16 'PRE'  [ ] P 'POST' [ tz ] Q" :=
-     (NDmk_funspec (nil, tz) cc_default (t1*t2*t3*t4*t5*t6*t7*t8*t9*t10*t11*t12*t13*t14*t15*t16)
+     (mk_funspec' (nil, tz) cc_default (t1*t2*t3*t4*t5*t6*t7*t8*t9*t10*t11*t12*t13*t14*t15*t16)
            (fun x => match x with (x1,x2,x3,x4,x5,x6,x7,x8,x9,x10,x11,x12,x13,x14,x15,x16) => P%assert end)
            (fun x => match x with (x1,x2,x3,x4,x5,x6,x7,x8,x9,x10,x11,x12,x13,x14,x15,x16) => Q%assert end))
             (at level 200, x1 at level 0, x2 at level 0, x3 at level 0, x4 at level 0,
@@ -259,7 +259,7 @@ Notation "'WITH'  x1 : t1 , x2 : t2 , x3 : t3 , x4 : t4 , x5 : t5 , x6 : t6 , x7
 
 
 Notation "'WITH'  x1 : t1 , x2 : t2 , x3 : t3 , x4 : t4 , x5 : t5 , x6 : t6 , x7 : t7 , x8 : t8 , x9 : t9 , x10 : t10 , x11 : t11 , x12 : t12 , x13 : t13 , x14 : t14 , x15 : t15 , x16 : t16 'PRE'  [ u , .. , v ] P 'POST' [ tz ] Q" :=
-     (NDmk_funspec ((cons u%formals .. (cons v%formals nil) ..), tz) cc_default (t1*t2*t3*t4*t5*t6*t7*t8*t9*t10*t11*t12*t13*t14*t15*t16)
+     (mk_funspec' ((cons u%formals .. (cons v%formals nil) ..), tz) cc_default (t1*t2*t3*t4*t5*t6*t7*t8*t9*t10*t11*t12*t13*t14*t15*t16)
            (fun x => match x with (x1,x2,x3,x4,x5,x6,x7,x8,x9,x10,x11,x12,x13,x14,x15,x16) => P%assert end)
            (fun x => match x with (x1,x2,x3,x4,x5,x6,x7,x8,x9,x10,x11,x12,x13,x14,x15,x16) => Q%assert end))
             (at level 200, x1 at level 0, x2 at level 0, x3 at level 0, x4 at level 0,
@@ -269,7 +269,7 @@ Notation "'WITH'  x1 : t1 , x2 : t2 , x3 : t3 , x4 : t4 , x5 : t5 , x6 : t6 , x7
              P at level 100, Q at level 100) : old_funspec_scope.
 
 Notation "'WITH'  x1 : t1 , x2 : t2 , x3 : t3 , x4 : t4 , x5 : t5 , x6 : t6 , x7 : t7 , x8 : t8 , x9 : t9 , x10 : t10 , x11 : t11 , x12 : t12 , x13 : t13 , x14 : t14 , x15 : t15 , x16 : t16 , x17 : t17 'PRE'  [ ] P 'POST' [ tz ] Q" :=
-     (NDmk_funspec (nil, tz) cc_default (t1*t2*t3*t4*t5*t6*t7*t8*t9*t10*t11*t12*t13*t14*t15*t16*t17)
+     (mk_funspec' (nil, tz) cc_default (t1*t2*t3*t4*t5*t6*t7*t8*t9*t10*t11*t12*t13*t14*t15*t16*t17)
            (fun x => match x with (x1,x2,x3,x4,x5,x6,x7,x8,x9,x10,x11,x12,x13,x14,x15,x16,x17) => P%assert end)
            (fun x => match x with (x1,x2,x3,x4,x5,x6,x7,x8,x9,x10,x11,x12,x13,x14,x15,x16,x17) => Q%assert end))
             (at level 200, x1 at level 0, x2 at level 0, x3 at level 0, x4 at level 0,
@@ -280,7 +280,7 @@ Notation "'WITH'  x1 : t1 , x2 : t2 , x3 : t3 , x4 : t4 , x5 : t5 , x6 : t6 , x7
 
 
 Notation "'WITH'  x1 : t1 , x2 : t2 , x3 : t3 , x4 : t4 , x5 : t5 , x6 : t6 , x7 : t7 , x8 : t8 , x9 : t9 , x10 : t10 , x11 : t11 , x12 : t12 , x13 : t13 , x14 : t14 , x15 : t15 , x16 : t16 , x17 : t17 'PRE'  [ u , .. , v ] P 'POST' [ tz ] Q" :=
-     (NDmk_funspec ((cons u%formals .. (cons v%formals nil) ..), tz) cc_default (t1*t2*t3*t4*t5*t6*t7*t8*t9*t10*t11*t12*t13*t14*t15*t16*t17)
+     (mk_funspec' ((cons u%formals .. (cons v%formals nil) ..), tz) cc_default (t1*t2*t3*t4*t5*t6*t7*t8*t9*t10*t11*t12*t13*t14*t15*t16*t17)
            (fun x => match x with (x1,x2,x3,x4,x5,x6,x7,x8,x9,x10,x11,x12,x13,x14,x15,x16,x17) => P%assert end)
            (fun x => match x with (x1,x2,x3,x4,x5,x6,x7,x8,x9,x10,x11,x12,x13,x14,x15,x16,x17) => Q%assert end))
             (at level 200, x1 at level 0, x2 at level 0, x3 at level 0, x4 at level 0,
@@ -290,7 +290,7 @@ Notation "'WITH'  x1 : t1 , x2 : t2 , x3 : t3 , x4 : t4 , x5 : t5 , x6 : t6 , x7
              P at level 100, Q at level 100) : old_funspec_scope.
 
 Notation "'WITH'  x1 : t1 , x2 : t2 , x3 : t3 , x4 : t4 , x5 : t5 , x6 : t6 , x7 : t7 , x8 : t8 , x9 : t9 , x10 : t10 , x11 : t11 , x12 : t12 , x13 : t13 , x14 : t14 , x15 : t15 , x16 : t16 , x17 : t17 , x18 : t18 'PRE'  [ ] P 'POST' [ tz ] Q" :=
-     (NDmk_funspec (nil, tz) cc_default (t1*t2*t3*t4*t5*t6*t7*t8*t9*t10*t11*t12*t13*t14*t15*t16*t17*t18)
+     (mk_funspec' (nil, tz) cc_default (t1*t2*t3*t4*t5*t6*t7*t8*t9*t10*t11*t12*t13*t14*t15*t16*t17*t18)
            (fun x => match x with (x1,x2,x3,x4,x5,x6,x7,x8,x9,x10,x11,x12,x13,x14,x15,x16,x17,x18) => P%assert end)
            (fun x => match x with (x1,x2,x3,x4,x5,x6,x7,x8,x9,x10,x11,x12,x13,x14,x15,x16,x17,x18) => Q%assert end))
             (at level 200, x1 at level 0, x2 at level 0, x3 at level 0, x4 at level 0,
@@ -301,7 +301,7 @@ Notation "'WITH'  x1 : t1 , x2 : t2 , x3 : t3 , x4 : t4 , x5 : t5 , x6 : t6 , x7
 
 
 Notation "'WITH'  x1 : t1 , x2 : t2 , x3 : t3 , x4 : t4 , x5 : t5 , x6 : t6 , x7 : t7 , x8 : t8 , x9 : t9 , x10 : t10 , x11 : t11 , x12 : t12 , x13 : t13 , x14 : t14 , x15 : t15 , x16 : t16 , x17 : t17 , x18 : t18 'PRE'  [ u , .. , v ] P 'POST' [ tz ] Q" :=
-     (NDmk_funspec ((cons u%formals .. (cons v%formals nil) ..), tz) cc_default (t1*t2*t3*t4*t5*t6*t7*t8*t9*t10*t11*t12*t13*t14*t15*t16*t17*t18)
+     (mk_funspec' ((cons u%formals .. (cons v%formals nil) ..), tz) cc_default (t1*t2*t3*t4*t5*t6*t7*t8*t9*t10*t11*t12*t13*t14*t15*t16*t17*t18)
            (fun x => match x with (x1,x2,x3,x4,x5,x6,x7,x8,x9,x10,x11,x12,x13,x14,x15,x16,x17,x18) => P%assert end)
            (fun x => match x with (x1,x2,x3,x4,x5,x6,x7,x8,x9,x10,x11,x12,x13,x14,x15,x16,x17,x18) => Q%assert end))
             (at level 200, x1 at level 0, x2 at level 0, x3 at level 0, x4 at level 0,
@@ -311,7 +311,7 @@ Notation "'WITH'  x1 : t1 , x2 : t2 , x3 : t3 , x4 : t4 , x5 : t5 , x6 : t6 , x7
              P at level 100, Q at level 100) : old_funspec_scope.
 
 Notation "'WITH'  x1 : t1 , x2 : t2 , x3 : t3 , x4 : t4 , x5 : t5 , x6 : t6 , x7 : t7 , x8 : t8 , x9 : t9 , x10 : t10 , x11 : t11 , x12 : t12 , x13 : t13 , x14 : t14 , x15 : t15 , x16 : t16 , x17 : t17 , x18 : t18 , x19 : t19 'PRE'  [ ] P 'POST' [ tz ] Q" :=
-     (NDmk_funspec (nil, tz) cc_default (t1*t2*t3*t4*t5*t6*t7*t8*t9*t10*t11*t12*t13*t14*t15*t16*t17*t18*t19)
+     (mk_funspec' (nil, tz) cc_default (t1*t2*t3*t4*t5*t6*t7*t8*t9*t10*t11*t12*t13*t14*t15*t16*t17*t18*t19)
            (fun x => match x with (x1,x2,x3,x4,x5,x6,x7,x8,x9,x10,x11,x12,x13,x14,x15,x16,x17,x18,x19) => P%assert end)
            (fun x => match x with (x1,x2,x3,x4,x5,x6,x7,x8,x9,x10,x11,x12,x13,x14,x15,x16,x17,x18,x19) => Q%assert end))
             (at level 200, x1 at level 0, x2 at level 0, x3 at level 0, x4 at level 0,
@@ -322,7 +322,7 @@ Notation "'WITH'  x1 : t1 , x2 : t2 , x3 : t3 , x4 : t4 , x5 : t5 , x6 : t6 , x7
 
 
 Notation "'WITH'  x1 : t1 , x2 : t2 , x3 : t3 , x4 : t4 , x5 : t5 , x6 : t6 , x7 : t7 , x8 : t8 , x9 : t9 , x10 : t10 , x11 : t11 , x12 : t12 , x13 : t13 , x14 : t14 , x15 : t15 , x16 : t16 , x17 : t17 , x18 : t18 , x19 : t19 'PRE'  [ u , .. , v ] P 'POST' [ tz ] Q" :=
-     (NDmk_funspec ((cons u%formals .. (cons v%formals nil) ..), tz) cc_default (t1*t2*t3*t4*t5*t6*t7*t8*t9*t10*t11*t12*t13*t14*t15*t16*t17*t18*t19)
+     (mk_funspec' ((cons u%formals .. (cons v%formals nil) ..), tz) cc_default (t1*t2*t3*t4*t5*t6*t7*t8*t9*t10*t11*t12*t13*t14*t15*t16*t17*t18*t19)
            (fun x => match x with (x1,x2,x3,x4,x5,x6,x7,x8,x9,x10,x11,x12,x13,x14,x15,x16,x17,x18,x19) => P%assert end)
            (fun x => match x with (x1,x2,x3,x4,x5,x6,x7,x8,x9,x10,x11,x12,x13,x14,x15,x16,x17,x18,x19) => Q%assert end))
             (at level 200, x1 at level 0, x2 at level 0, x3 at level 0, x4 at level 0,
@@ -332,7 +332,7 @@ Notation "'WITH'  x1 : t1 , x2 : t2 , x3 : t3 , x4 : t4 , x5 : t5 , x6 : t6 , x7
              P at level 100, Q at level 100) : old_funspec_scope.
 
 Notation "'WITH'  x1 : t1 , x2 : t2 , x3 : t3 , x4 : t4 , x5 : t5 , x6 : t6 , x7 : t7 , x8 : t8 , x9 : t9 , x10 : t10 , x11 : t11 , x12 : t12 , x13 : t13 , x14 : t14 , x15 : t15 , x16 : t16 , x17 : t17 , x18 : t18 , x19 : t19 , x20 : t20 'PRE'  [ ] P 'POST' [ tz ] Q" :=
-     (NDmk_funspec (nil, tz) cc_default (t1*t2*t3*t4*t5*t6*t7*t8*t9*t10*t11*t12*t13*t14*t15*t16*t17*t18*t19*t20)
+     (mk_funspec' (nil, tz) cc_default (t1*t2*t3*t4*t5*t6*t7*t8*t9*t10*t11*t12*t13*t14*t15*t16*t17*t18*t19*t20)
            (fun x => match x with (x1,x2,x3,x4,x5,x6,x7,x8,x9,x10,x11,x12,x13,x14,x15,x16,x17,x18,x19,x20) => P%assert end)
            (fun x => match x with (x1,x2,x3,x4,x5,x6,x7,x8,x9,x10,x11,x12,x13,x14,x15,x16,x17,x18,x19,x20) => Q%assert end))
             (at level 200, x1 at level 0, x2 at level 0, x3 at level 0, x4 at level 0,
@@ -344,7 +344,7 @@ Notation "'WITH'  x1 : t1 , x2 : t2 , x3 : t3 , x4 : t4 , x5 : t5 , x6 : t6 , x7
 
 
 Notation "'WITH'  x1 : t1 , x2 : t2 , x3 : t3 , x4 : t4 , x5 : t5 , x6 : t6 , x7 : t7 , x8 : t8 , x9 : t9 , x10 : t10 , x11 : t11 , x12 : t12 , x13 : t13 , x14 : t14 , x15 : t15 , x16 : t16 , x17 : t17 , x18 : t18 , x19 : t19 , x20 : t20 'PRE'  [ u , .. , v ] P 'POST' [ tz ] Q" :=
-     (NDmk_funspec ((cons u%formals .. (cons v%formals nil) ..), tz) cc_default (t1*t2*t3*t4*t5*t6*t7*t8*t9*t10*t11*t12*t13*t14*t15*t16*t17*t18*t19*t20)
+     (mk_funspec' ((cons u%formals .. (cons v%formals nil) ..), tz) cc_default (t1*t2*t3*t4*t5*t6*t7*t8*t9*t10*t11*t12*t13*t14*t15*t16*t17*t18*t19*t20)
            (fun x => match x with (x1,x2,x3,x4,x5,x6,x7,x8,x9,x10,x11,x12,x13,x14,x15,x16,x17,x18,x19,x20) => P%assert end)
            (fun x => match x with (x1,x2,x3,x4,x5,x6,x7,x8,x9,x10,x11,x12,x13,x14,x15,x16,x17,x18,x19,x20) => Q%assert end))
             (at level 200, x1 at level 0, x2 at level 0, x3 at level 0, x4 at level 0,
@@ -355,7 +355,7 @@ Notation "'WITH'  x1 : t1 , x2 : t2 , x3 : t3 , x4 : t4 , x5 : t5 , x6 : t6 , x7
              P at level 100, Q at level 100) : old_funspec_scope.
 
 Notation "'WITH'  x1 : t1 , x2 : t2 , x3 : t3 , x4 : t4 , x5 : t5 , x6 : t6 , x7 : t7 , x8 : t8 , x9 : t9 , x10 : t10 , x11 : t11 , x12 : t12 , x13 : t13 , x14 : t14 , x15 : t15 , x16 : t16 , x17 : t17 , x18 : t18 , x19 : t19 , x20 : t20 , x21 : t21 'PRE'  [ ] P 'POST' [ tz ] Q" :=
-     (NDmk_funspec (nil, tz) cc_default (t1*t2*t3*t4*t5*t6*t7*t8*t9*t10*t11*t12*t13*t14*t15*t16*t17*t18*t19*t20*t21)
+     (mk_funspec' (nil, tz) cc_default (t1*t2*t3*t4*t5*t6*t7*t8*t9*t10*t11*t12*t13*t14*t15*t16*t17*t18*t19*t20*t21)
            (fun x => match x with (x1,x2,x3,x4,x5,x6,x7,x8,x9,x10,x11,x12,x13,x14,x15,x16,x17,x18,x19,x20,x21) => P%assert end)
            (fun x => match x with (x1,x2,x3,x4,x5,x6,x7,x8,x9,x10,x11,x12,x13,x14,x15,x16,x17,x18,x19,x20,x21) => Q%assert end))
             (at level 200, x1 at level 0, x2 at level 0, x3 at level 0, x4 at level 0,
@@ -367,7 +367,7 @@ Notation "'WITH'  x1 : t1 , x2 : t2 , x3 : t3 , x4 : t4 , x5 : t5 , x6 : t6 , x7
 
 
 Notation "'WITH'  x1 : t1 , x2 : t2 , x3 : t3 , x4 : t4 , x5 : t5 , x6 : t6 , x7 : t7 , x8 : t8 , x9 : t9 , x10 : t10 , x11 : t11 , x12 : t12 , x13 : t13 , x14 : t14 , x15 : t15 , x16 : t16 , x17 : t17 , x18 : t18 , x19 : t19 , x20 : t20 , x21 : t21 'PRE'  [ u , .. , v ] P 'POST' [ tz ] Q" :=
-     (NDmk_funspec ((cons u%formals .. (cons v%formals nil) ..), tz) cc_default (t1*t2*t3*t4*t5*t6*t7*t8*t9*t10*t11*t12*t13*t14*t15*t16*t17*t18*t19*t20*t21)
+     (mk_funspec' ((cons u%formals .. (cons v%formals nil) ..), tz) cc_default (t1*t2*t3*t4*t5*t6*t7*t8*t9*t10*t11*t12*t13*t14*t15*t16*t17*t18*t19*t20*t21)
            (fun x => match x with (x1,x2,x3,x4,x5,x6,x7,x8,x9,x10,x11,x12,x13,x14,x15,x16,x17,x18,x19,x20,x21) => P%assert end)
            (fun x => match x with (x1,x2,x3,x4,x5,x6,x7,x8,x9,x10,x11,x12,x13,x14,x15,x16,x17,x18,x19,x20,x21) => Q%assert end))
             (at level 200, x1 at level 0, x2 at level 0, x3 at level 0, x4 at level 0,
@@ -378,7 +378,7 @@ Notation "'WITH'  x1 : t1 , x2 : t2 , x3 : t3 , x4 : t4 , x5 : t5 , x6 : t6 , x7
              P at level 100, Q at level 100) : old_funspec_scope.
 
 Notation "'WITH'  x1 : t1 , x2 : t2 , x3 : t3 , x4 : t4 , x5 : t5 , x6 : t6 , x7 : t7 , x8 : t8 , x9 : t9 , x10 : t10 , x11 : t11 , x12 : t12 , x13 : t13 , x14 : t14 , x15 : t15 , x16 : t16 , x17 : t17 , x18 : t18 , x19 : t19 , x20 : t20 , x21 : t21 , x22 : t22 'PRE'  [ ] P 'POST' [ tz ] Q" :=
-     (NDmk_funspec (nil, tz) cc_default (t1*t2*t3*t4*t5*t6*t7*t8*t9*t10*t11*t12*t13*t14*t15*t16*t17*t18*t19*t20*t21*t22)
+     (mk_funspec' (nil, tz) cc_default (t1*t2*t3*t4*t5*t6*t7*t8*t9*t10*t11*t12*t13*t14*t15*t16*t17*t18*t19*t20*t21*t22)
            (fun x => match x with (x1,x2,x3,x4,x5,x6,x7,x8,x9,x10,x11,x12,x13,x14,x15,x16,x17,x18,x19,x20,x21,x22) => P%assert end)
            (fun x => match x with (x1,x2,x3,x4,x5,x6,x7,x8,x9,x10,x11,x12,x13,x14,x15,x16,x17,x18,x19,x20,x21,x22) => Q%assert end))
             (at level 200, x1 at level 0, x2 at level 0, x3 at level 0, x4 at level 0,
@@ -390,7 +390,7 @@ Notation "'WITH'  x1 : t1 , x2 : t2 , x3 : t3 , x4 : t4 , x5 : t5 , x6 : t6 , x7
 
 
 Notation "'WITH'  x1 : t1 , x2 : t2 , x3 : t3 , x4 : t4 , x5 : t5 , x6 : t6 , x7 : t7 , x8 : t8 , x9 : t9 , x10 : t10 , x11 : t11 , x12 : t12 , x13 : t13 , x14 : t14 , x15 : t15 , x16 : t16 , x17 : t17 , x18 : t18 , x19 : t19 , x20 : t20 , x21 : t21 , x22 : t22 'PRE'  [ u , .. , v ] P 'POST' [ tz ] Q" :=
-     (NDmk_funspec ((cons u%formals .. (cons v%formals nil) ..), tz) cc_default (t1*t2*t3*t4*t5*t6*t7*t8*t9*t10*t11*t12*t13*t14*t15*t16*t17*t18*t19*t20*t21*t22)
+     (mk_funspec' ((cons u%formals .. (cons v%formals nil) ..), tz) cc_default (t1*t2*t3*t4*t5*t6*t7*t8*t9*t10*t11*t12*t13*t14*t15*t16*t17*t18*t19*t20*t21*t22)
            (fun x => match x with (x1,x2,x3,x4,x5,x6,x7,x8,x9,x10,x11,x12,x13,x14,x15,x16,x17,x18,x19,x20,x21,x22) => P%assert end)
            (fun x => match x with (x1,x2,x3,x4,x5,x6,x7,x8,x9,x10,x11,x12,x13,x14,x15,x16,x17,x18,x19,x20,x21,x22) => Q%assert end))
             (at level 200, x1 at level 0, x2 at level 0, x3 at level 0, x4 at level 0,
@@ -422,8 +422,6 @@ iSplit.
   iDestruct "G" as %->; auto.
 - iIntros "((% & %) & $)"; subst; auto.
 Qed.
-
-Ltac rewrite_old_main_pre ::= rewrite ?old_main_pre_eq; unfold convertPre.
 
 (*Notation "'main_pre'" := (old_main_pre) : old_funspec_scope. *)
 (*
@@ -548,81 +546,6 @@ Lemma nullval_neq_Vundef: nullval <> Vundef.
 Proof.
 intro; inv H.
 Qed.
-
-Ltac prove_all_defined := 
- red; simpl makePARAMS;
-lazymatch goal with |- ⌜ ?A _ _ _⌝ ∧ _ ⊢ ⌜?B⌝ =>
- let a := fresh "a" in let b := fresh "b" in 
-  set (b:=B); set (a:=A); 
-  unfold fold_right in a;
- simpl in b;
-  unfold fold_right_sepcon;
-  subst a b; cbv beta iota zeta
-end;
-pull_out_props;
-saturate_local;
-apply bi.pure_intro; repeat split;
-let H := fresh in 
-try congruence; 
-try apply Vptrofs_neq_Vundef;
-try apply Vbyte_neq_Vundef;
-try apply nullval_neq_Vundef;
-try (intro H; rewrite H in *;
-      (contradiction || eapply field_compatible_Vundef; eassumption));
-match goal with  |- ?A <> Vundef =>
-  fail 100 "From assumptions above the line and PROP and SEP clauses in precondition, cannot prove LOCAL variable" A "<>Vundef"
-end.
-
-Ltac convertPreElim' := 
-unfold convertPre;
-let ae := fresh "ae" in split => ae;
-let g := fresh "g" in let args := fresh "args" in destruct ae as [g args];
-lazymatch goal with |-
-  _ ∧ (PROPx _ (LOCALx ?Q _) _)  ⊣⊢  PROPx _ (LAMBDAx ?G _ _) _ =>
- unify G (globals_localdefs Q)
-end;
-apply convertPre_helper2;
- [intro;
-  simpl fst; simpl snd;
-  match goal with |- ⌜_ = Datatypes.length ?L⌝ ∧ local (fold_right _ _ (map _ ?D)) _ ⊣⊢
-                              ⌜args = ?A⌝ ∧ local (fold_right _ _ (map _ (map _ ?G))) _ => 
-  let p := constr:(makePARAMS L D) in
-  let p := eval simpl in p in 
-    unify A p
-   end
-  | ];
-  [ | prove_all_defined ];
-unfold local, lift1; unfold_lift; rewrite -!bi.pure_and; f_equiv;
-let H0 := fresh in let H1 := fresh  in
-apply prop_ext; split; intros [H0 H1];
-[ simpl in H0;
-  repeat (destruct args as [ | ? args]; [discriminate H0 | ]);
-  destruct args; [clear H0 | inv H0];
-  simpl in H1; unfold_lift in H1;
-  unfold eval_id, env_set in H1;
-  simpl in H1; 
-  decompose [and] H1; clear H1; subst;
-  simpl;
-  repeat split; auto
-| subst args; 
-  simpl in H1; unfold_lift in H1;
-  unfold eval_id, env_set in H1;
-  simpl in H1; 
-  decompose [and] H1; clear H1; subst;
-  simpl; unfold_lift; unfold eval_id, env_set; simpl;
-  repeat match goal with H: Forall _ _ |- _ => inv H end;
-  repeat split; auto
-].
-
-Ltac convertPreElim := 
-  match goal with |- convertPre _ _ _ _ = _ => idtac end;
-  convertPreElim' || fail 100 "Could not convert old-style precondition to new-style".
-
-Ltac try_convertPreElim ::= 
-  lazymatch goal with
-  | |- convertPre _ _ _ _ = _ =>  convertPreElim
-  | |- _ => reflexivity
-  end.
 
 Lemma convertPre_helper3:
   forall (fsig: funsig) P Q R vals gvs,
@@ -855,6 +778,84 @@ rewrite H1; clear H1.
 *)
 Admitted. (* might be true *)
 
+End mpred.
+
+Ltac rewrite_old_main_pre ::= rewrite ?old_main_pre_eq; unfold convertPre.
+
+Ltac prove_all_defined := 
+ red; simpl makePARAMS;
+lazymatch goal with |- ⌜ ?A _ _ _⌝ ∧ _ ⊢ ⌜?B⌝ =>
+ let a := fresh "a" in let b := fresh "b" in 
+  set (b:=B); set (a:=A); 
+  unfold fold_right in a;
+ simpl in b;
+  unfold fold_right_sepcon;
+  subst a b; cbv beta iota zeta
+end;
+pull_out_props;
+saturate_local;
+apply bi.pure_intro; repeat split;
+let H := fresh in 
+try congruence; 
+try apply Vptrofs_neq_Vundef;
+try apply Vbyte_neq_Vundef;
+try apply nullval_neq_Vundef;
+try (intro H; rewrite H in *;
+      (contradiction || eapply field_compatible_Vundef; eassumption));
+match goal with  |- ?A <> Vundef =>
+  fail 100 "From assumptions above the line and PROP and SEP clauses in precondition, cannot prove LOCAL variable" A "<>Vundef"
+end.
+
+Ltac convertPreElim' := 
+unfold convertPre;
+let ae := fresh "ae" in split => ae;
+let g := fresh "g" in let args := fresh "args" in destruct ae as [g args];
+lazymatch goal with |-
+  _ ∧ (PROPx _ (LOCALx ?Q _) _)  ⊣⊢  PROPx _ (LAMBDAx ?G _ _) _ =>
+ unify G (globals_localdefs Q)
+end;
+apply convertPre_helper2;
+ [intro;
+  simpl fst; simpl snd;
+  match goal with |- ⌜_ = Datatypes.length ?L⌝ ∧ local (fold_right _ _ (map _ ?D)) _ ⊣⊢
+                              ⌜args = ?A⌝ ∧ local (fold_right _ _ (map _ (map _ ?G))) _ => 
+  let p := constr:(makePARAMS L D) in
+  let p := eval simpl in p in 
+    unify A p
+   end
+  | ];
+  [ | prove_all_defined ];
+unfold local, lift1; unfold_lift; rewrite -!bi.pure_and; f_equiv;
+let H0 := fresh in let H1 := fresh  in
+apply prop_ext; split; intros [H0 H1];
+[ simpl in H0;
+  repeat (destruct args as [ | ? args]; [discriminate H0 | ]);
+  destruct args; [clear H0 | inv H0];
+  simpl in H1; unfold_lift in H1;
+  unfold eval_id, env_set in H1;
+  simpl in H1; 
+  decompose [and] H1; clear H1; subst;
+  simpl;
+  repeat split; auto
+| subst args; 
+  simpl in H1; unfold_lift in H1;
+  unfold eval_id, env_set in H1;
+  simpl in H1; 
+  decompose [and] H1; clear H1; subst;
+  simpl; unfold_lift; unfold eval_id, env_set; simpl;
+  repeat match goal with H: Forall _ _ |- _ => inv H end;
+  repeat split; auto
+].
+
+Ltac convertPreElim := 
+  match goal with |- convertPre _ _ _ _ = _ => idtac end;
+  convertPreElim' || fail 100 "Could not convert old-style precondition to new-style".
+
+Ltac try_convertPreElim ::= 
+  lazymatch goal with
+  | |- convertPre _ _ _ _ = _ =>  convertPreElim
+  | |- _ => reflexivity
+  end.
 
 Ltac prove_norepet := 
    clear; repeat constructor; simpl; intros ?H;
