progs/list_dt.v
@@ -1446,47 +1446,46 @@ Qed.
 
 
 Lemma semax_lseg_nonnull (ls: listspec list_structid list_link list_token):
-  forall (Espec: OracleKind)
-      Delta P Q sh s v R c Post,
+  forall Espec
+      E Delta P Q sh s v R c Post,
       ENTAIL Delta, PROPx P (LOCALx Q
             (SEPx (lseg ls sh s v nullval :: R))) |--
                         !!(typed_true (tptr list_struct) v)  ->
   (forall (h: elemtype ls) (r: list (elemtype ls)) (y: val),
     s=h::r -> is_pointer_or_null y ->
-    semax Delta
+    semax(OK_spec := Espec) E Delta
         (PROPx P (LOCALx Q
         (SEPx (list_token sh v :: list_cell ls sh h v ::
                   field_at sh list_struct (StructField list_link :: nil) (valinject (nested_field_type list_struct (StructField list_link :: nil)) y) v ::
                    lseg ls sh r y nullval ::
                   R)))) c Post) ->
-   semax Delta
+   semax E Delta
        (PROPx P (LOCALx Q (SEPx (lseg ls sh s v nullval :: R))))
        c Post.
 Proof.
 intros.
 assert_PROP (~ ptr_eq v nullval).
-eapply derives_trans; [apply H |].
+rewrite H.
 normalize.
 apply semax_lseg_neq; auto.
 Qed.
 
 Lemma lseg_nil_eq (ls: listspec list_structid list_link list_token):
-    forall sh p q, lseg ls sh nil p q = !! (ptr_eq p q) && emp.
+    forall sh p q, lseg ls sh nil p q ⊣⊢ !! (ptr_eq p q) && emp.
 Proof. intros.
  rewrite lseg_unroll.
  apply pred_ext.
- apply bi.or_elim.
- rewrite andp_assoc.
- apply andp_derives; auto.
-rewrite prop_true_andp by auto. auto.
- unfold lseg_cons. normalize. inv H0.
- apply bi.or_intro_l.  rewrite andp_assoc.
- rewrite (prop_true_andp (_ = _)) by auto. auto.
+ - apply bi.or_elim.
+   + rewrite <- bi.pure_and.
+     apply bi.pure_elim_l; intros []; auto.
+   + unfold lseg_cons. normalize. inv H0.
+ - rewrite <- bi.or_intro_l.
+   apply bi.pure_elim_l; intros; auto.
 Qed.
 
 Lemma lseg_cons_eq (ls: listspec list_structid list_link list_token):
      forall sh h r x z ,
-    lseg ls sh (h::r) x z =
+    lseg ls sh (h::r) x z ⊣⊢
         !!(~ ptr_eq x z) &&
          (EX  y : val,
           !!(is_pointer_or_null y) &&
@@ -1495,21 +1494,16 @@ Lemma lseg_cons_eq (ls: listspec list_structid list_link list_token):
 Proof.
  intros. rewrite lseg_unroll.
  apply pred_ext.
- apply bi.or_elim.
- rewrite andp_assoc.
- apply bi.pure_elim_l; intro.
- apply bi.pure_elim_l; intro.
- inv H0.
- unfold lseg_cons.
- normalize.
- symmetry in H0; inv H0.
- apply bi.exist_intro with y. normalize.
- apply bi.or_intro_r.
- unfold lseg_cons.
- apply andp_derives; auto.
- apply bi.exist_intro with h. apply bi.exist_intro with r.  apply bi.exist_mono; intro y.
- normalize.
-  autorewrite with subst norm1 norm2; normalize.
+ - apply bi.or_elim.
+   + rewrite <- bi.pure_and.
+     apply bi.pure_elim_l; intros []; discriminate.
+   + unfold lseg_cons. normalize. inv H0.
+     Exists y; entailer!.
+ - rewrite <- bi.or_intro_r.
+   Intros y.
+   unfold lseg_cons.
+   apply bi.and_intro; first auto.
+   Exists h r y; entailer!.
 Qed.
 
 Definition lseg_cons_right (ls: listspec list_structid list_link list_token)
@@ -1530,10 +1524,9 @@ Proof.
 intros.
 unfold lseg.
 normalize.
-apply bi.exist_intro with (al ++ (y,h)::nil).
+Exists (al ++ (y,h)::nil).
 rewrite prop_true_andp by (rewrite map_app; reflexivity).
-eapply derives_trans; [ | apply LsegGeneral.lseg_cons_right_neq; auto].
-cancel.
+apply LsegGeneral.lseg_cons_right_neq; auto.
 Qed.
 
 Lemma lseg_cons_right_null (ls: listspec list_structid list_link list_token): forall sh l x h y,
@@ -1544,10 +1537,9 @@ Proof.
 intros.
 unfold lseg.
 normalize.
-apply bi.exist_intro with (al ++ (y,h)::nil).
+Exists (al ++ (y,h)::nil).
 rewrite prop_true_andp by (rewrite map_app; reflexivity).
-eapply derives_trans; [ | apply LsegGeneral.lseg_cons_right_null].
-cancel.
+apply LsegGeneral.lseg_cons_right_null.
 Qed.
 
 
@@ -1561,20 +1553,14 @@ intros.
 destruct l'.
 rewrite lseg_nil_eq.
 normalize.
-rewrite prop_true_andp by apply ptr_eq_nullval.
-apply lseg_cons_right_null.
+rewrite lseg_cons_right_null; auto.
 rewrite lseg_cons_eq.
 Intros u.
 Exists u.
 rewrite !prop_true_andp by auto.
-rewrite <- !sepcon_assoc.
-apply bi.sep_mono; auto.
-pull_right (list_cell ls sh e z).
-pull_right (list_token sh z).
-apply bi.sep_mono; auto.
-apply bi.sep_mono; auto.
-apply lseg_cons_right_neq.
-auto.
+iIntros "(H & (? & Hz) & ?)".
+iDestruct (lseg_cons_right_neq with "[$H $Hz]") as "($ & $)"; first done.
+iFrame.
 Qed.
 
 Lemma lseg_unroll_right (ls: listspec list_structid list_link list_token): forall sh l x z ,
@@ -1589,7 +1575,7 @@ Proof.
 intros.
 unfold lseg.
 normalize.
-eapply derives_trans; [apply LsegGeneral.lseg_local_facts |].
+rewrite LsegGeneral.lseg_local_facts.
 normalize.
 split; auto.
 rewrite H.
@@ -1605,7 +1591,7 @@ Definition lseg_cell (ls: listspec list_structid list_link list_token)
 Lemma lseg_cons_eq2: forall
   (ls : listspec list_structid list_link list_token) (sh : share) (h : elemtype ls)
    (r : list (elemtype ls))
-  (x z : val), lseg ls sh (h :: r) x z =
+  (x z : val), lseg ls sh (h :: r) x z ⊣⊢
   !!(~ ptr_eq x z) && (EX  y : val, lseg_cell ls sh h x y * lseg ls sh r y z).
 Proof.
   intros.
@@ -1623,13 +1609,10 @@ Proof.
   intros.
   unfold lseg.
  normalize.
- eapply derives_trans.
- apply LsegGeneral.list_append.
- intros.
- eapply derives_trans; [ | apply (H x0 tl')].
+ rewrite LsegGeneral.list_append; [ | intros; apply (H _ tl')].
  unfold lseg_cell, LsegGeneral.lseg_cell.
  entailer.
- apply bi.exist_intro with (x++al).
+ Exists (al++a).
  rewrite prop_true_andp; auto.
  rewrite map_app; reflexivity.
 Qed.
@@ -1643,9 +1626,9 @@ Lemma list_append_null:
    lseg ls sh (ct1++ct2) hd nullval.
 Proof.
 intros.
- rewrite <- sepcon_emp.
- eapply derives_trans; [ | apply (list_append hd mid nullval ct1 ct2 (fun _ => emp))].
- normalize.
+ rewrite <- bi.sep_emp.
+ rewrite (list_append _ _ _ _ _ (fun _ => emp)).
+ iIntros "($ & _)".
  intros.
   unfold lseg_cell. simpl. saturate_local. destruct H. contradiction H.
 Qed.
@@ -1661,15 +1644,13 @@ Proof.
   intros ? ? ? ? NON_ID ?.
  rewrite list_cell_link_join_nospacer; auto.
  unfold data_at_, field_at_, data_at.
- eapply derives_trans; [ apply field_at_valid_ptr; auto | ].
+ saturate_local.
+ rewrite field_at_valid_ptr; auto.
+ 2: {
  change (nested_field_type list_struct nil) with list_struct.
- apply LsegGeneral.sizeof_list_struct_pos.
+ apply LsegGeneral.sizeof_list_struct_pos. }
  unfold field_address.
- if_tac; auto.
- change (Int.repr (nested_field_offset list_struct nil)) with Int.zero.
-  rewrite valid_pointer_offset_val_zero; auto.
- simpl.
- change predicates_hered.False with False. apply False_left.
+ if_tac; auto; contradiction.
 Qed.
 
 Lemma lseg_valid_pointer:
@@ -1682,20 +1663,16 @@ Lemma lseg_valid_pointer:
 Proof.
 intros ? ? ? ? ? ? NON_ID ? ?.
 destruct contents.
-rewrite lseg_nil_eq. normalize.
+rewrite lseg_nil_eq, H0; entailer!.
 unfold lseg; simpl.
-normalize.
+Intros al.
 destruct al; inv H1.
 rewrite LsegGeneral.lseg_cons_eq.
-normalize.
-destruct p0 as [p z]; simpl in *.
-apply sepcon_valid_pointer2.
-apply sepcon_valid_pointer1.
-rewrite sepcon_assoc.
-apply sepcon_valid_pointer2.
-eapply derives_trans; [ | eapply list_cell_valid_pointer; eauto].
-apply bi.sep_mono ; [ apply derives_refl | ].
-cancel.
+Intros y.
+subst; destruct p0 as [p z]; simpl in *.
+iIntros "(? & ((? & cell) & Hp) & ?)".
+iPoseProof (list_cell_valid_pointer with "[$cell Hp]") as "$"; auto.
+iStopProof; cancel.
 Qed.
 
 End LIST.
@@ -1708,7 +1685,7 @@ Ltac resolve_lseg_valid_pointer :=
 match goal with
  | |- ?Q |-- valid_pointer ?p =>
    match Q with context [lseg ?A ?B ?C p ?q] =>
-   repeat rewrite <- sepcon_assoc;
+   repeat rewrite bi.sep_assoc;
    pull_right (lseg A B C p q);
    apply lseg_valid_pointer; [auto | reflexivity | ];
    auto 50 with valid_pointer
@@ -1748,12 +1725,12 @@ Definition lseg (ls: listspec list_structid list_link list_token) (dsh psh: shar
 Lemma nonreadable_list_cell_eq:
   forall (ls: listspec list_structid list_link list_token) sh v v' p,
     ~ readable_share sh ->
-   list_cell ls sh v p = list_cell ls sh v' p.
+   list_cell ls sh v p ⊣⊢ list_cell ls sh v' p.
 Proof.
 unfold list_cell; intros.
  destruct (field_compatible_dec list_struct nil p);
     [ | solve [ apply pred_ext; normalize ]].
- f_equal.
+ f_equiv.
  revert v v'; unfold elemtype.
  set (m := all_but_link list_fields).
  assert (PLAIN: plain_members m = true). {
@@ -1774,12 +1751,12 @@ unfold list_cell; intros.
  clear IHm; simpl.
  Transparent field_type field_offset.
  rewrite !withspacer_spacer.
- f_equal.
+ f_equiv.
  admit. (* apply nonreadable_data_at_rec_eq; auto. *) (* list_cell should be defined by field_at instead of data_at_rec. *)
  +
  rewrite !struct_pred_cons2.
  rewrite !withspacer_spacer.
- f_equal. f_equal.
+ f_equiv. f_equiv.
  * admit. (* unfold at_offset. apply nonreadable_data_at_rec_eq; auto.*)
  * apply IHm.
    simpl; auto. 
@@ -1788,14 +1765,13 @@ Admitted.
 Lemma cell_share_join:
   forall (ls: listspec list_structid list_link list_token) ash bsh psh p v,
    sepalg.join ash bsh psh ->
-   list_cell ls ash v p * list_cell ls bsh v p = list_cell ls psh v p.
+   list_cell ls ash v p * list_cell ls bsh v p ⊣⊢ list_cell ls psh v p.
 Proof.
  intros.
  unfold list_cell.
  destruct (field_compatible_dec list_struct nil p);
     [ | solve [ apply pred_ext; normalize ]].
  normalize.
- f_equal.
  revert v; unfold elemtype.
  set (m := all_but_link list_fields).
  assert (PLAIN: plain_members m = true). {
@@ -1806,7 +1782,7 @@ Proof.
  }
  clearbody m.
  induction m; intros.
- simpl. rewrite emp_sepcon; auto.
+ simpl. apply bi.emp_sep.
  destruct a as [i t|]; [ | discriminate].
  assert (field_compatible (field_type i list_fields) nil
   (offset_val (field_offset cenv_cs i list_fields) p))
@@ -1814,7 +1790,7 @@ Proof.
  destruct m as [ | [i' t'|]]; [ | | discriminate].
  +
  clear IHm; simpl. rewrite !withspacer_spacer.
- rewrite <- sepcon_assoc.
+(* rewrite assoc.
  match goal with |- ?A * ?B * ?C * ?D = _ =>
     pull_left C; pull_left A
  end.
@@ -1842,7 +1818,7 @@ Proof.
  assert (isptr p) by (auto with field_compatible).
  destruct p; try inversion H1.
  apply data_at_rec_share_join; auto.
- apply IHm. auto.
+ apply IHm. auto.*)
 Admitted.
 
 Lemma join_cell_link (ls: listspec list_structid list_link list_token):
@@ -1850,7 +1826,7 @@ Lemma join_cell_link (ls: listspec list_structid list_link list_token):
    sepalg.join ash bsh psh ->
   ~ (readable_share ash) ->
     readable_share bsh ->
-   list_cell ls ash v' p * list_cell ls bsh v p = list_cell ls psh v p.
+   list_cell ls ash v' p * list_cell ls bsh v p ⊣⊢ list_cell ls psh v p.
  Proof.
  intros.
  rewrite (nonreadable_list_cell_eq _ _ v' v _ H0).
@@ -1878,13 +1854,13 @@ Qed.
 Lemma lseg_eq (ls: listspec list_structid list_link list_token):
   forall dsh psh l v ,
   is_pointer_or_null v ->
-    lseg ls dsh psh l v v = !!(l=nil) && emp.
+    lseg ls dsh psh l v v ⊣⊢ !!(l=nil) && emp.
 Proof.
 intros.
 rewrite (lseg_unfold ls dsh psh l v v).
 destruct l.
-f_equal. f_equal.
-apply prop_ext; split; intro; auto.
+f_equiv. f_equiv.
+split; intro; auto.
 normalize.
 apply pred_ext;
 apply bi.pure_elim_l; intro.
@@ -1906,7 +1882,7 @@ Definition lseg_cons (ls: listspec list_structid list_link list_token) dsh psh
 
 Lemma lseg_unroll (ls: listspec list_structid list_link list_token): forall dsh psh l x z ,
     ~ (readable_share dsh) ->
-    lseg ls dsh psh l x z =
+    lseg ls dsh psh l x z ⊣⊢
       (!! (ptr_eq x z) && !! (l=nil) && emp) || lseg_cons ls dsh psh l x z.
 Proof.
 intros.
@@ -1917,48 +1893,31 @@ apply bi.pure_elim_l; intros.
 rewrite prop_true_andp by auto.
 rewrite prop_true_andp by auto.
 apply bi.or_intro_l; auto.
-apply bi.or_intro_r.
+rewrite <- bi.or_intro_r.
 unfold lseg_cons.
 apply bi.pure_elim_l; intros.
 destruct H.
 subst x.
 apply bi.exist_elim; intro tail.
 rewrite (prop_true_andp (~ptr_eq v z)) by auto.
-apply bi.exist_intro with (vund ls).
-apply bi.exist_intro with l.
-apply bi.exist_intro with tail.
+Exists (vund ls) l tail.
 normalize.
-  autorewrite with subst norm1 norm2; normalize.
 apply bi.or_elim.
-rewrite andp_assoc;
-do 2 (apply bi.pure_elim_l; intro).
- rewrite prop_true_andp by auto. auto.
+rewrite <- bi.pure_and; apply bi.pure_elim_l; intros [].
+auto.
 unfold lseg_cons.
-apply bi.pure_elim_l; intros.
-apply bi.exist_elim; intro h.
-apply bi.exist_elim; intro r.
-apply bi.exist_elim; intro y.
-do 3 rewrite sepcon_andp_prop'.
-apply bi.pure_elim_l; intros [? ?].
+Intros h r y.
 inv H0.
 apply bi.or_elim.
-rewrite andp_assoc;
-do 2 (apply bi.pure_elim_l; intro).
+rewrite <- bi.pure_and; apply bi.pure_elim_l; intros [].
 inv H0.
 unfold lseg_cons.
-apply bi.pure_elim_l; intros.
-apply bi.exist_elim; intro h.
-apply bi.exist_elim; intro r.
-apply bi.exist_elim; intro y.
-do 3 rewrite sepcon_andp_prop'.
-apply bi.pure_elim_l; intros [? ?].
+Intros h r y.
 symmetry in H0; inv H0.
  rewrite prop_true_andp by auto.
-apply bi.exist_intro with y.
-normalize.
-repeat (apply bi.sep_mono; auto).
-clear - NR.
-apply derives_refl'; apply nonreadable_list_cell_eq; auto.
+Exists y.
+entailer!.
+rewrite nonreadable_list_cell_eq; auto.
 Qed.
 
 Lemma lseg_unroll_nonempty1 (ls: listspec list_structid list_link list_token):
@@ -1971,33 +1930,31 @@ Lemma lseg_unroll_nonempty1 (ls: listspec list_structid list_link list_token):
                    (valinject (nested_field_type list_struct (StructField list_link :: nil)) p) v1 *
                lseg ls dsh psh tail p v2)) ->
     P |-- lseg ls dsh psh (v1::tail) v1 v2.
-Proof. intros. rewrite lseg_unroll by auto. apply bi.or_intro_r. unfold lseg_cons.
+Proof. intros. rewrite lseg_unroll by auto. rewrite <- bi.or_intro_r. unfold lseg_cons.
   rewrite prop_true_andp by auto.
-  apply bi.exist_intro with h. apply bi.exist_intro with tail. apply bi.exist_intro with p.
+  Exists h tail p.
     rewrite prop_true_andp by auto.
- rewrite sepcon_assoc.
- eapply derives_trans; [ eassumption | ].
- apply bi.sep_mono; auto.
+  rewrite H2; cancel.
 Qed.
 
 Lemma lseg_neq (ls: listspec list_structid list_link list_token):
   forall dsh psh s v v2,
     ~ (readable_share dsh) ->
     ptr_neq v v2 ->
-     lseg ls dsh psh s v v2 = lseg_cons ls dsh psh s v v2.
+     lseg ls dsh psh s v v2 ⊣⊢ lseg_cons ls dsh psh s v v2.
+Proof.
 intros. rewrite lseg_unroll by auto.
 apply pred_ext. apply bi.or_elim; auto.
-rewrite andp_assoc.
-do 2 (apply bi.pure_elim_l; intro).
+rewrite <- bi.pure_and; apply bi.pure_elim_l; intros [].
 congruence.
-apply bi.or_intro_r. auto.
+apply bi.or_intro_r.
 Qed.
 
 Lemma lseg_nonnull (ls: listspec list_structid list_link list_token):
   forall dsh psh s v,
     ~ (readable_share dsh) ->
       typed_true (tptr list_struct) v ->
-     lseg ls dsh psh s v nullval = lseg_cons ls dsh psh s v nullval.
+     lseg ls dsh psh s v nullval ⊣⊢ lseg_cons ls dsh psh s v nullval.
 Proof.
 intros. unfold nullval.
 apply lseg_neq; auto.
@@ -2025,35 +1982,29 @@ Lemma unfold_lseg_neq (ls: listspec list_structid list_link list_token):
         end.
 Proof.
 intros.
-apply derives_trans with
+trans
 (PROPx P (LOCALx (Q1::Q) (SEPx (lseg_cons ls dsh psh s v v2 :: R)))).
-apply derives_trans with
+trans
 (!! (ptr_neq v v2) && PROPx P (LOCALx (Q1::Q) (SEPx (lseg ls dsh psh s v v2 :: R)))).
 apply bi.and_intro; auto.
-intro rho; unfold PROPx,LOCALx,SEPx,local,tc_expr,tc_lvalue; unfold_lift; simpl.
+split => rho; unfold PROPx,LOCALx,SEPx,local,tc_expr,tc_lvalue; unfold_lift; simpl; monPred.unseal.
 unfold lift1; simpl.
  repeat (apply bi.pure_elim_l; intro).
  rewrite prop_true_andp by auto.
  rewrite prop_true_andp by auto.
 apply bi.sep_mono; auto.
 rewrite lseg_neq; auto.
-intro rho; unfold PROPx,LOCALx,SEPx,local,tc_expr,tc_lvalue,lift2,lift1,lift0; simpl.
+split => rho; unfold PROPx,LOCALx,SEPx,local,tc_expr,tc_lvalue,lift2,lift1,lift0; simpl; monPred.unseal.
  unfold_lift.
  unfold lseg_cons. simpl.
  apply bi.pure_elim_l; intro.
  apply bi.pure_elim_l; intros [? ?].
  rewrite sepcon_andp_prop'.
  apply bi.pure_elim_l; intro.
- rewrite exp_sepcon1; apply bi.exist_elim; intro h.
- rewrite exp_sepcon1; apply bi.exist_elim; intro r.
- rewrite exp_sepcon1; apply bi.exist_elim; intro y.
+ Intros h r y.
  repeat rewrite sepcon_andp_prop'.
- apply bi.pure_elim_l; intros [? ?].
- subst.
- apply bi.exist_intro with (h,r,y, v).
- repeat rewrite prop_true_andp by auto.
- repeat rewrite sepcon_assoc.
- auto.
+ subst; simpl.
+ Exists (h, r, y, v); simpl; entailer!.
 Qed.
 
 Lemma unfold_lseg_cons (ls: listspec list_structid list_link list_token):
@@ -2074,8 +2025,7 @@ Lemma unfold_lseg_cons (ls: listspec list_structid list_link list_token):
         end.
 Proof.
 intros. apply unfold_lseg_neq; auto.
-eapply derives_trans.
-apply H0. normalize.
+rewrite H0. normalize.
 unfold local. super_unfold_lift.
 unfold nullval. destruct e; inv H1; try congruence; auto.
 intro. apply ptr_eq_e in H1.
@@ -2083,20 +2033,20 @@ destruct Archi.ptr64; inv H1.
 Qed.
 
 Lemma semax_lseg_neq (ls: listspec list_structid list_link list_token):
-  forall (Espec: OracleKind)
-      Delta P Q dsh psh s v v2 R c Post,
+  forall Espec
+      E Delta P Q dsh psh s v v2 R c Post,
     ~ (readable_share dsh) ->
     ~ (ptr_eq v v2) ->
   (forall (h: elemtype ls) (r: list val) (y: val),
     s=v::r -> is_pointer_or_null y ->
-    semax Delta
+    semax(OK_spec := Espec) E Delta
         (PROPx P (LOCALx Q
         (SEPx (list_token dsh v :: list_cell ls dsh h v ::
                   field_at psh list_struct (StructField list_link :: nil)
                       (valinject (nested_field_type list_struct (StructField list_link :: nil)) y) v ::
                   lseg ls dsh psh r y v2 ::
                   R)))) c Post) ->
-   semax Delta
+   semax E Delta
        (PROPx P (LOCALx Q (SEPx (lseg ls dsh psh s v v2 :: R))))
        c Post.
 Proof.
@@ -2114,9 +2064,7 @@ apply semax_pre0 with
         lseg ls dsh psh r y v2 :: R)))).
 go_lowerx; entailer.
 Exists h r y.
-rewrite <- ?sepcon_assoc.
-normalize.
-  autorewrite with subst norm1 norm2; normalize.
+entailer!.
 Intros h r y.
 apply semax_extract_prop; intros [? ?].
 eauto.
@@ -2124,27 +2072,27 @@ Qed.
 
 
 Lemma semax_lseg_nonnull (ls: listspec list_structid list_link list_token):
-  forall (Espec: OracleKind)
-      Delta P Q dsh psh s v R c Post,
+  forall Espec
+      E Delta P Q dsh psh s v R c Post,
     ~ (readable_share dsh) ->
    ENTAIL Delta, PROPx P (LOCALx Q
             (SEPx (lseg ls dsh psh s v nullval :: R))) |--
                         !!(typed_true (tptr list_struct) v)  ->
   (forall (h: elemtype ls) (r: list val) (y: val),
     s=v::r -> is_pointer_or_null y ->
-    semax Delta
+    semax(OK_spec := Espec) E Delta
         (PROPx P (LOCALx Q
         (SEPx (list_token dsh v :: list_cell ls dsh h v ::
                   field_at psh list_struct (StructField list_link :: nil) (valinject (nested_field_type list_struct (StructField list_link :: nil)) y) v ::
                   lseg ls dsh psh r y nullval ::
                   R)))) c Post) ->
-   semax Delta
+   semax E Delta
        (PROPx P (LOCALx Q (SEPx (lseg ls dsh psh s v nullval :: R))))
        c Post.
 Proof.
 intros.
 assert_PROP (~ ptr_eq v nullval).
-eapply derives_trans; [eapply H0 |].
+rewrite H0.
 normalize.
 apply semax_lseg_neq; auto.
 Qed.
@@ -2159,7 +2107,7 @@ Qed.
 Lemma lseg_cons_eq (ls: listspec list_structid list_link list_token):
      forall dsh psh h r x z ,
      ~ (readable_share dsh) ->
-    lseg ls dsh psh (h::r) x z =
+    lseg ls dsh psh (h::r) x z ⊣⊢
         !!(x = h /\ ~ ptr_eq x z) &&
          (EX  y : val,
           !!(is_pointer_or_null y) &&
@@ -2169,24 +2117,18 @@ Proof.
  intros. rewrite lseg_unroll by auto.
  apply pred_ext.
  apply bi.or_elim.
- rewrite andp_assoc.
- apply bi.pure_elim_l; intro.
- apply bi.pure_elim_l; intro.
+ Intros.
  inv H1.
  unfold lseg_cons.
- normalize.
+ Intros h0 r0 y.
  symmetry in H1; inv H1.
- apply bi.exist_intro with y. normalize.
-  autorewrite with subst norm1 norm2; normalize.
- repeat (apply bi.sep_mono; auto).
- apply derives_refl'; apply nonreadable_list_cell_eq; auto.
- apply bi.or_intro_r.
- normalize.
+ Exists y; entailer!.
+ rewrite nonreadable_list_cell_eq; auto.
+ rewrite <- bi.or_intro_r.
+ Intros y.
  unfold lseg_cons.
  rewrite prop_true_andp by auto.
- apply bi.exist_intro with (vund ls). apply bi.exist_intro with r.  apply bi.exist_intro with y.
- normalize.
-  autorewrite with subst norm1 norm2; normalize.
+ Exists (vund ls) r y; entailer!.
 Qed.
 
 Definition lseg_cons_right (ls: listspec list_structid list_link list_token)
@@ -2210,34 +2152,22 @@ intros. rename H into SH. rename H0 into NR.
 assert (SZ: 0 < sizeof (nested_field_type list_struct (DOT list_link)))
   by (rewrite list_link_type; unfold sizeof; simpl; destruct Archi.ptr64; computable).
 rewrite (field_at_isptr _ _ _ _ z).
-normalize.
+Intros.
 revert x; induction l; simpl; intros.
 *
 unfold lseg.
 simpl.
-normalize.
-  autorewrite with subst norm1 norm2; normalize.
-apply bi.exist_intro with z.
-entailer.
- apply derives_refl';  f_equal. f_equal. f_equal.
- apply (nonreadable_list_cell_eq); auto.
+Intros; subst.
+Exists z.
+entailer!.
+rewrite (nonreadable_list_cell_eq); auto.
 *
 unfold lseg; simpl.
-normalize.
-apply bi.exist_intro with x0.
-rewrite <- ?sepcon_assoc.
-normalize.
-  autorewrite with subst norm1 norm2; normalize.
-specialize (IHl x0).
-entailer.
-pull_right (list_token dsh x); pull_right (list_cell ls dsh (vund ls) x).
-apply bi.sep_mono; auto.
-apply bi.sep_mono; auto.
-pull_right (field_at psh list_struct (StructField list_link :: nil)
-      (valinject
-         (nested_field_type list_struct (StructField list_link :: nil)) x0)
-      x).
-apply bi.sep_mono; auto.
+Intros x0; Exists x0.
+iIntros "((H & ? & lseg) & Hz)".
+iDestruct (IHl with "[$H $Hz $lseg]") as "?".
+iStopProof; entailer!.
+auto.
 Qed.
 
 Lemma lseg_cons_right_null (ls: listspec list_structid list_link list_token): forall dsh psh l x h y,
@@ -2250,36 +2180,15 @@ intros. rename H into NR.
 unfold lseg.
 revert x; induction l; simpl; intros.
 *
-normalize.
-  autorewrite with subst norm1 norm2; normalize.
-apply bi.exist_intro with nullval.
-apply bi.and_intro.
-apply not_bi.pure_intro; intro.
-apply ptr_eq_e in H. subst y.
-entailer!.
-destruct H. contradiction H.
-rewrite prop_true_andp by reflexivity.
-rewrite prop_true_andp by apply ptr_eq_nullval.
-normalize.
-apply derives_refl'; f_equal. f_equal.
-apply nonreadable_list_cell_eq; auto.
+Intros.
+Exists nullval; entailer!.
+rewrite nonreadable_list_cell_eq; auto.
 *
-normalize.
-apply bi.exist_intro with x0.
-normalize.
-  autorewrite with subst norm1 norm2; normalize.
-specialize (IHl x0).
-apply bi.and_intro.
-rewrite prop_and.
-apply bi.and_intro; [ | apply bi.pure_intro; auto].
-apply not_bi.pure_intro; intro.
-apply ptr_eq_e in H0. subst x.
-entailer.
-destruct H2; contradiction H2.
-eapply derives_trans.
-2: apply bi.sep_mono; [ | eassumption]; apply derives_refl.
-clear IHl.
-cancel.
+Intros x0.
+Exists x0.
+iIntros "(H & ? & lseg)".
+iDestruct (IHl with "[$H $lseg]") as "$".
+iStopProof; entailer!.
 Qed.
 
 
@@ -2294,19 +2203,15 @@ Proof.
 intros.
 destruct l'.
 rewrite lseg_nil_eq.
-normalize.
+Intros; subst.
 rewrite prop_true_andp by apply ptr_eq_nullval.
-apply lseg_cons_right_null; auto.
+rewrite lseg_cons_right_null; auto.
 rewrite lseg_cons_eq; auto.
 Intros u. Exists u. subst.
 rewrite !prop_true_andp by auto.
-rewrite <- !sepcon_assoc.
-apply bi.sep_mono; auto.
-pull_right (list_cell ls dsh (vund ls) v).
-apply bi.sep_mono; auto.
-pull_right (list_token dsh v).
-apply bi.sep_mono; auto.
-apply lseg_cons_right_neq; auto.
+iIntros "(H & ((? & ?) & Hv) & ?)".
+iDestruct (lseg_cons_right_neq with "[$H $Hv]") as "?"; auto.
+iStopProof; cancel.
 Qed.
 
 Lemma lseg_unroll_right (ls: listspec list_structid list_link list_token): forall sh sh' l x z ,
@@ -2326,27 +2231,25 @@ unfold ptr_eq in H.
 apply bi.pure_intro.
 destruct p; try contradiction; simpl; auto.
 destruct q; try contradiction; auto.
-destruct H as [? [? ?]]. rewrite H.
-unfold Int.cmpu in *.
+unfold Int.cmpu in H.
+destruct H as [? [? ?]].
 apply int_eq_e in H0.
 apply int_eq_e in H1. subst.
 split; auto; split; auto.
 destruct q; try contradiction; auto.
-destruct H as [? [? ?]]. rewrite H.
-unfold Int64.cmpu in *.
+unfold Int64.cmpu in H.
+destruct H as [? [? ?]].
 apply int64_eq_e in H0.
 apply int64_eq_e in H1. subst.
-split; auto; split; auto.
-destruct q; try contradiction; auto.
+split3; auto; done.
+destruct q; try contradiction.
 destruct H; subst.
-unfold Ptrofs.cmpu in *.
-apply ptrofs_eq_e in H0. subst.
-intuition.
+unfold Ptrofs.cmpu in H0.
+apply ptrofs_eq_e in H0.
+subst. tauto.
 normalize.
 rewrite field_at_isptr.
-normalize.
-  autorewrite with subst norm1 norm2; normalize.
-apply bi.pure_intro.
+Intros; entailer!.
 split. intro; subst q.
 contradiction H. normalize.
 intros. discriminate.
@@ -2361,16 +2264,15 @@ Lemma lseg_cons_eq2: forall
   (ls : listspec list_structid list_link list_token) (dsh psh : share) (h : elemtype ls)
    (r : list val )  (x z : val),
      ~ (readable_share dsh) ->
-  lseg ls dsh psh (x :: r) x z =
+  lseg ls dsh psh (x :: r) x z ⊣⊢
   !!(~ ptr_eq x z) && (EX  y : val, lseg_cell ls dsh psh h x y * lseg ls dsh psh r y z).
 Proof.
   intros.
   rewrite -> lseg_cons_eq by auto.
   unfold lseg_cell.
  normalize.
-  autorewrite with subst norm1 norm2; normalize.
- f_equal. extensionality y.
- f_equal. f_equal. f_equal. f_equal.
+ f_equiv. intros y.
+ f_equiv. f_equiv. tauto. f_equiv. f_equiv. f_equiv.
  apply nonreadable_list_cell_eq; auto.
 Qed.
 
@@ -2386,33 +2288,20 @@ Proof.
 *
  normalize.
 *
- normalize.
- progress (autorewrite with subst norm1 norm2); normalize.
- apply bi.exist_intro with y.
+ Intros y.
+ Exists y.
  apply bi.and_intro.
  +
-  apply not_bi.pure_intro; intro. apply ptr_eq_e in H1; subst hd.
+  destruct (eq_dec hd tl); [|entailer!].
+  subst.
   clear IHct1.
   specialize (H y).
   unfold lseg_cell in H.
-  rewrite prop_true_andp in H by auto.
-  change (LsegGeneral.lseg ls dsh psh (map (fun v : val => (v, vund ls)) ct1))
-    with (lseg ls dsh psh ct1).
-  change (LsegGeneral.lseg ls dsh psh (map (fun v : val => (v, vund ls)) ct2))
-    with (lseg ls dsh psh ct2).
-  apply derives_trans with
-        (lseg ls dsh psh ct1 y mid * lseg ls dsh psh ct2 mid tl * False).
-  cancel. auto.
-  rewrite sepcon_False; auto.
+  iIntros "(((H & ?) & ?) & P)"; iDestruct (H with "[H $P]") as "[]".
+  iStopProof; entailer!.
  +
-  normalize.
-  specialize (IHct1 y). clear H.
-   do 2 rewrite sepcon_assoc.
-  eapply derives_trans.
- apply bi.sep_mono.
-  apply derives_refl.
-  rewrite <- !sepcon_assoc; eassumption.
-  cancel.
+  rewrite <- !bi.sep_assoc, <- IHct1.
+  entailer!.
 Qed.
 
 Lemma list_append_null:
@@ -2424,9 +2313,9 @@ Lemma list_append_null:
    lseg ls dsh psh (ct1++ct2) hd nullval.
 Proof.
 intros.
- rewrite <- sepcon_emp.
- eapply derives_trans; [ | apply (list_append hd mid nullval ct1 ct2 (fun _ => emp))].
- normalize.
+ rewrite <- bi.sep_emp.
+ rewrite (list_append _ _ _ _ _ (fun _ => emp)).
+ iIntros "($ & _)".
  intros.
   unfold lseg_cell. simpl. saturate_local. destruct H. contradiction H.
 Qed.
@@ -2443,19 +2332,17 @@ Proof.
   intros ? ? ? ? ? NON_ID ? ?.
  destruct H as [bsh ?].
  rewrite <- (field_at__share_join _ _ _ _ _ _ H).
- rewrite <- sepcon_assoc.
- rewrite list_cell_link_join_nospacer; auto.
- apply sepcon_valid_pointer1.
+ iIntros "(c & f & _)".
+ iCombine "c f" as "d"; rewrite list_cell_link_join_nospacer; auto.
  unfold data_at_, field_at_, data_at.
- eapply derives_trans; [ apply field_at_valid_ptr; auto | ].
- change (nested_field_type list_struct nil) with list_struct.
- apply LsegGeneral.sizeof_list_struct_pos.
+ iStopProof.
+ saturate_local.
+ rewrite field_at_valid_ptr; auto.
+ 2: { change (nested_field_type list_struct nil) with list_struct.
+      apply LsegGeneral.sizeof_list_struct_pos. }
  unfold field_address.
  if_tac; auto.
- change (Int.repr (nested_field_offset list_struct nil)) with Int.zero.
-  rewrite valid_pointer_offset_val_zero; auto.
- simpl.
- change predicates_hered.False with False. apply False_left.
+ contradiction.
 Qed.
 
 Lemma list_cell_valid_pointerx:
@@ -2480,18 +2367,12 @@ Lemma lseg_valid_pointer:
 Proof.
 intros.
 destruct contents.
-rewrite lseg_nil_eq. normalize.
+rewrite lseg_nil_eq, H3. entailer!.
 unfold lseg; simpl.
-normalize.
-apply sepcon_valid_pointer2.
-rewrite !sepcon_assoc.
-apply sepcon_valid_pointer2.
-rewrite <- !sepcon_assoc.
-apply sepcon_valid_pointer1.
-eapply derives_trans with
-  (list_cell ls dsh (vund  ls) p * field_at_ psh list_struct (StructField list_link :: nil) p).
-cancel.
-apply list_cell_valid_pointer; auto.
+Intros y.
+iIntros "(? & ((? & cell) & Hp) & ?)".
+iPoseProof (list_cell_valid_pointer with "[$cell Hp]") as "$"; eauto.
+iStopProof; cancel.
 Qed.
 
 End LIST2.
@@ -2513,7 +2394,7 @@ Ltac resolve_lseg_valid_pointer :=
 match goal with
  | |- ?Q |-- valid_pointer ?p =>
    match Q with context [lseg ?A ?B ?C ?D p ?q] =>
-   repeat rewrite <- sepcon_assoc;
+   repeat rewrite bi.sep_assoc;
    pull_right (lseg A B C D p q);
    apply lseg_valid_pointer; [auto | | | reflexivity | ];
    auto 50 with valid_pointer
@@ -2527,9 +2408,9 @@ Ltac resolve_list_cell_valid_pointer :=
  match goal with |- ?A |-- valid_pointer ?p =>
   match A with context [@list_cell ?cs ?sid ?lid ?tok ?LS ?dsh ?v p] =>
    match A with context [field_at ?psh ?t (StructField lid::nil) ?v' p] =>
-    apply derives_trans with
+    trans
       (@list_cell cs sid lid tok LS dsh v p *
-      field_at_ psh t (StructField lid::nil) p * TT);
+      field_at_ psh t (StructField lid::nil) p * True);
       [cancel
       | apply sepcon_valid_pointer1;
         apply list_cell_valid_pointer; [auto | | reflexivity]; auto with valid_pointer]
