progs/verif_min.v
@@ -274,6 +274,4 @@ forward_if.
  Intros x.
  autorewrite with sublist in *.
  forward. (* return *)
- Exists x.
- entailer!!.
 Qed.
