progs/verif_nest2.v
@@ -5,8 +5,6 @@ Require Import VST.progs.nest2.
 #[export] Instance CompSpecs : compspecs. make_compspecs prog. Defined.
 Definition Vprog : varspecs. mk_varspecs prog. Defined.
 
-Local Open Scope logic.
-
 Definition t_struct_b := Tstruct _b noattr.
 
 Definition get_spec :=
@@ -76,4 +74,3 @@ unfold_repinj.
 Time forward. (* 1.23 sec *)
 entailer!!.
 Time Qed.  (*  28 sec -> 3.45 sec *)
-
