progs/verif_queue.v
@@ -1,9 +1,8 @@
 Require Import VST.floyd.proofauto.
+Require Import VST.floyd.compat.
 Require Import VST.floyd.library.
 Require Import VST.progs.list_dt. Import Links.
 Require Import VST.progs.queue.
-
-Open Scope logic.
 
 #[export] Instance CompSpecs : compspecs. make_compspecs prog. Defined.
 Definition Vprog : varspecs. mk_varspecs prog. Defined.
