sha/spec_sha.v
@@ -9,7 +9,6 @@ Require Import VST.floyd.Funspec_old_Notation.
 
 #[export] Instance CompSpecs : compspecs. make_compspecs prog. Defined.
 Definition Vprog : varspecs. mk_varspecs prog. Defined.
-Open Scope logic.
 
 Definition s256state := (list val * (val * (val * (list val * val))))%type.
 Definition s256_h (s: s256state) := fst s.
